Test/VProg.v
@@ -10,9 +10,9 @@ Section Program.
 
 
 Definition spec_0 : FDecl (ptr * ptr) _ unit _
-  FOR (p0, p1)
-  FOR (n0, n1) [] [vptr p0 ~> n0; vptr p1 ~> n1] True
-  RET _ FOR tt [vptr p0 ~> n1; vptr p1 ~> n0] True.
+  SPEC (p0, p1)
+  '(n0, n1) [] [vptr p0 ~> n0; vptr p1 ~> n1] True
+  '_ tt [vptr p0 ~> n1; vptr p1 ~> n0] True.
 Proof. Derived. Defined.
 Variable f_0 : spec_0 CT.
 
@@ -22,28 +22,28 @@ Definition vprog_0 : FImpl f_0 := fun '(p0, p1) =>
   Write p0 v1;;
   Write p1 v0.
 Lemma correct_0 : FCorrect vprog_0.
-Proof. by_wlp. Qed.
+Proof. solve_by_wlp. Qed.
 
 
 Definition spec_1 : FDecl (ptr * ptr * ptr) _ unit _
-  FOR (p0, p1, p2)
-  FOR (n0, n1, n2) [vptr p2 ~> n2] [vptr p0 ~> n0; vptr p1 ~> n1] True
-  RET _ FOR tt [vptr p0 ~> n1; vptr p1 ~> n0] True.
+  SPEC (p0, p1, p2)
+  '(n0, n1, n2) [vptr p2 ~> n2] [vptr p0 ~> n0; vptr p1 ~> n1] True
+  '_ tt [vptr p0 ~> n1; vptr p1 ~> n0] True.
 Proof. Derived. Defined.
 Variable f_1 : spec_1 CT.
 
 Definition vprog_1 : FImpl f_1 := fun '(p0, p1, p2) =>
   f_0 (p0, p1).
 Lemma correct_1 : FCorrect vprog_1.
-Proof. by_wlp. Qed.
+Proof. solve_by_wlp. Qed.
 
 
 Definition data42 : nat := 42.
 
 Definition spec_2 : FDecl (ptr * ptr * ptr) _ ptr _
-  FOR (p0, p1, p2)
-  FOR (n0, n1, n2) [vptr p2 ~> n2] [vptr p0 ~> n0; vptr p1 ~> n1] True
-  RET p FOR (n, n1') [vptr p ~> n; vptr p1 ~> n1'] (n1' > 0).
+  SPEC (p0, p1, p2)
+  '(n0, n1, n2) [vptr p2 ~> n2] [vptr p0 ~> n0; vptr p1 ~> n1] True
+  'p (n, n1') [vptr p ~> n; vptr p1 ~> n1'] (n1' > 0).
 Proof. Derived. Defined.
 Variable f_2 : spec_2 CT.
 
@@ -55,28 +55,28 @@ Definition vprog_2 : FImpl f_2 := fun '(p0, p1, p2) =>
   Ret p0 (pt := fun p => [vptr p ~>]).
 Lemma correct_2: FCorrect vprog_2.
 Proof.
-  by_wlp.
+  solve_by_wlp.
   unfold data42; repeat constructor.
 Qed.
 
 
 Definition spec_3 : FDecl ptr (Some (fun _ => ptr)) ptr (Some (fun _ => ptr))
-  FOR p0 & p1
-  FOR (n0, n1) [] [vptr p0 ~> n0; vptr p1 ~> n1] True
-  RET p0' & p1' FOR (n0', n1') [vptr p0' ~> n0'; vptr p1' ~> n1'] True.
+  SPEC p0 & p1
+  '(n0, n1) [] [vptr p0 ~> n0; vptr p1 ~> n1] True
+  'p0' & p1' (n0', n1') [vptr p0' ~> n0'; vptr p1' ~> n1'] True.
 Proof. Derived. Defined.
 Variable f_3 : spec_3 CT.
 
 Definition vprog_3 : FImpl f_3 := fun p0 p1 =>
   RetG p0 p1 (pt := fun p0 p1 => [vptr p0 ~>; vptr p1 ~>]).
 Lemma correct_3: FCorrect vprog_3.
-Proof. by_wlp. Qed.
+Proof. solve_by_wlp. Qed.
 
 
 Definition spec_4 : FDecl (ptr * ptr) _ ptr (Some (fun _ => ptr))
-  FOR (p0, p1)
-  FOR (n0, n1) [] [vptr p0 ~> n0; vptr p1 ~> n1] True
-  RET p0' & p1' FOR (n0', n1') [vptr p0' ~> n0'; vptr p1' ~> n1'] True.
+  SPEC (p0, p1)
+  '(n0, n1) [] [vptr p0 ~> n0; vptr p1 ~> n1] True
+  'p0' & p1' (n0', n1') [vptr p0' ~> n0'; vptr p1' ~> n1'] True.
 Proof. Derived. Defined.
 Variable f_4 : spec_4 CT.
 
@@ -84,36 +84,35 @@ Definition vprog_4 : FImpl f_4 := fun '(p0, p1) =>
   'p0' p1' <- f_3 p0 p1;
   RetG p0' p1' (pt := fun p0 p1 => [vptr p0 ~>; vptr p1 ~>]).
 Lemma correct_4: FCorrect vprog_4.
-Proof. by_wlp. Qed.
+Proof. solve_by_wlp. Qed.
 
 
 Definition cell2 (p : ptr) '(v0, v1) : SLprop.t :=
   (SLprop.cell p v0 ** SLprop.cell (S p) v1)%slprop.
 
 Definition elim_cell2_spec : LDecl ptr unit
-  FOR p FOR n01 [] [cell2 p ~> n01] True
-  RET _ FOR tt [vptr p ~> (fst n01); vptr (S p) ~> (snd n01)] True.
+  SPEC p 'n01 [] [cell2 p ~> n01] True
+  '_ tt [vptr p ~> (fst n01); vptr (S p) ~> (snd n01)] True.
 Proof. Derived. Defined.
 Lemma elim_cell2 : elim_cell2_spec.
 Proof.
-  init_lemma p (n0, n1) _.
+  init_lemma p (n0, n1) ?.
   reflexivity.
 Qed.
 
 Definition intro_cell2_spec : LDecl ptr unit
-  FOR p FOR (n0, n1) [] [vptr p ~> n0; vptr (S p) ~> n1] True
-  RET _ FOR tt [cell2 p ~> (n0, n1)] True.
+  SPEC p '(n0, n1) [] [vptr p ~> n0; vptr (S p) ~> n1] True
+  '_ tt [cell2 p ~> (n0, n1)] True.
 Proof. Derived. Defined.
 Lemma intro_cell2 : intro_cell2_spec.
 Proof.
-  init_lemma p (n0, n1) _.
+  init_lemma p (n0, n1) ?.
   reflexivity.
 Qed.
 
 Definition spec_5 : FDecl ptr _ unit _
-  FOR p
-  FOR v [] [cell2 p ~> v] True
-  RET _ FOR v' [cell2 p ~> v'] (v' = let (n0, n1) := v in (S n0, n1)).
+  SPEC p 'v [] [cell2 p ~> v] True
+  '_ v' [cell2 p ~> v'] (v' = let (n0, n1) := v in (S n0, n1)).
 Proof. Derived. Defined.
 Variable f_5 : spec_5 CT.
 
@@ -123,7 +122,7 @@ Definition vprog_5 : FImpl f_5 := fun p =>
   Write p (S n);;
   gLem intro_cell2 p.
 Lemma correct_5: FCorrect vprog_5.
-Proof. by_wlp. case sel0; reflexivity. Qed.
+Proof. solve_by_wlp. Qed.
 
 End Program.
 
@@ -142,9 +141,8 @@ Section Other.
 
 Definition sigh_a0 := mk_f_sig1 (ptr * ptr) None unit None.
 Definition spec_a0 : FSpec sigh_a0
-  FOR ps
-  FOR n [vptr (fst ps) ~> n] [] True
-  RET _ FOR tt [] True.
+  SPEC ps 'n [vptr (fst ps) ~> n] [] True
+  '_ tt [] True.
 Proof. Tac.build_FSpec. Defined.
 
 Definition vprog_a0 : f_body CT sigh_a0 := fun ps =>
@@ -152,7 +150,7 @@ Definition vprog_a0 : f_body CT sigh_a0 := fun ps =>
   Ret tt.
 Lemma imatch_a0:
   f_body_match vprog_a0 (m_spec spec_a0).
-Proof. by_wlp. Qed.
+Proof. solve_by_wlp. Qed.
 
 Definition cp_a0: f_extract vprog_a0.
 Proof. Tac.extract_impl. Defined.
@@ -160,9 +158,9 @@ Proof. Tac.extract_impl. Defined.
 
 Definition sigh_a1a := mk_f_sig1 (bool * ptr * ptr * ptr) None unit None.
 Definition spec_a1a : FSpec sigh_a1a
-  FOR (b, p0, p1, p2)
-  FOR (n0, n1, n2) [vptr p0 ~> n0] [vptr p1 ~> n1; vptr p2 ~> n2] True
-  RET _ FOR (n1', n2') [vptr p1 ~> n1'; vptr p2 ~> n2'] (b = true -> n1' = 0).
+  SPEC (b, p0, p1, p2)
+  '(n0, n1, n2) [vptr p0 ~> n0] [vptr p1 ~> n1; vptr p2 ~> n2] True
+  '_ (n1', n2') [vptr p1 ~> n1'; vptr p2 ~> n2'] (b = true -> n1' = 0).
 Proof. Tac.build_FSpec. Defined.
 
 Definition vprog_a1a : f_body CT sigh_a1a := fun '(b, p0, p1, p2) =>
@@ -171,7 +169,7 @@ Definition vprog_a1a : f_body CT sigh_a1a := fun '(b, p0, p1, p2) =>
   else Write p2 1.
 Lemma imatch_a1a:
   f_body_match vprog_a1a (m_spec spec_a1a).
-Proof. by_wlp; congruence. Qed.
+Proof. solve_by_wlp; congruence. Qed.
 
 Definition cp_a1a: f_extract vprog_a1a.
 Proof. Tac.extract_impl. Defined.
@@ -181,9 +179,9 @@ Inductive bool3 : Set := B0 | B1 | B2.
 
 Definition sigh_a1b := mk_f_sig1 (bool3 * ptr) None unit None.
 Definition spec_a1b : FSpec sigh_a1b
-  FOR (b, p)
-  FOR n [] [vptr p ~> n] (b <> B2)
-  RET _ FOR n' [vptr p ~> n'] (b <> B1 -> n' = 0).
+  SPEC (b, p)
+  'n [] [vptr p ~> n] (b <> B2)
+  '_ n' [vptr p ~> n'] (b <> B1 -> n' = 0).
 Proof. Tac.build_FSpec. Defined.
 
 Definition vprog_a1b : f_body CT sigh_a1b := fun '(b, p) =>
@@ -193,14 +191,14 @@ Definition vprog_a1b : f_body CT sigh_a1b := fun '(b, p) =>
   end.
 Lemma imatch_a1b:
   f_body_match vprog_a1b (m_spec spec_a1b).
-Proof. by_wlp; congruence. Qed.
+Proof. solve_by_wlp; congruence. Qed.
 
 
 Definition sigh_a1c := mk_f_sig1 (option nat * ptr) None unit None.
 Definition spec_a1c : FSpec sigh_a1c
-  FOR (o, p)
-  FOR n [] [vptr p ~> n] (n > 0 /\ match o with Some n' => n' > 0 | None => True end)
-  RET _ FOR n' [vptr p ~> n'] (n' > 0).
+  SPEC (o, p)
+  'n [] [vptr p ~> n] (n > 0 /\ match o with Some n' => n' > 0 | None => True end)
+  '_ n' [vptr p ~> n'] (n' > 0).
 Proof. Tac.build_FSpec. Defined.
 
 Definition vprog_a1c : f_body CT sigh_a1c := fun '(o, p) =>
@@ -210,14 +208,14 @@ Definition vprog_a1c : f_body CT sigh_a1c := fun '(o, p) =>
   end.
 Lemma imatch_a1c:
   f_body_match vprog_a1c (m_spec spec_a1c).
-Proof. by_wlp. Qed.
+Proof. solve_by_wlp. Qed.
 
 
 Definition sigh_a2a := mk_f_sig1 (ptr * ptr) None unit None.
 Definition spec_a2a : FSpec sigh_a2a
-  FOR (p0, p1)
-  FOR (n0, n1) [vptr p0 ~> n0] [vptr p1 ~> n1] (n0 <= n1)
-  RET _ FOR n1' [vptr p1 ~> n1'] (n0 <= n1').
+  SPEC (p0, p1)
+  '(n0, n1) [vptr p0 ~> n0] [vptr p1 ~> n1] (n0 <= n1)
+  '_ n1' [vptr p1 ~> n1'] (n0 <= n1').
 Proof. Tac.build_FSpec. Defined.
 
 Definition vprog_a2a : f_body CT sigh_a2a := fun '(p0, p1) =>
@@ -227,7 +225,7 @@ Definition vprog_a2a : f_body CT sigh_a2a := fun '(p0, p1) =>
   Write p1 (S v1).
 Lemma imatch_a2a:
   f_body_match vprog_a2a (m_spec spec_a2a).
-Proof. by_wlp. Qed.
+Proof. solve_by_wlp. Qed.
 Definition cp_a2a: f_extract vprog_a2a.
 Proof. Tac.extract_impl. Defined.
 
@@ -240,23 +238,23 @@ Definition vprog_a2b : f_body CT sigh_a2a := fun '(p0, p1) =>
   Write p1 (S v1).
 Lemma imatch_a2b:
   f_body_match vprog_a2b (m_spec spec_a2a).
-Proof. by_wlp. Qed.
+Proof. solve_by_wlp. Qed.
 Definition cp_a2b: f_extract vprog_a2b.
 Proof. Tac.extract_impl. Defined.
 
 
 Definition sigh_a3 := mk_f_sig1 unit (Some (fun _ => (nat * nat)%type <: Type)) unit (Some (fun _ => nat <: Type)).
 Definition spec_a3 : FSpec sigh_a3
-  FOR _ & (n0, n1)
-  FOR tt [] [] True
-  RET _ & r FOR tt [] (r = n0 + n1).
+  SPEC _ & (n0, n1)
+  'tt [] [] True
+  '_ & r tt [] (r = n0 + n1).
 Proof. Tac.build_FSpec. Defined.
 
 Definition vprog_a3 : f_body CT sigh_a3 := fun _ '(n0, n1) =>
   RetG tt (n0 + n1).
 Lemma imatch_a3:
   f_body_match vprog_a3 (m_spec spec_a3).
-Proof. by_wlp. Qed.
+Proof. solve_by_wlp. Qed.
 Definition cp_a3: f_extract vprog_a3.
 Proof. Tac.extract_impl. Defined.
 End Other.
